theories/L6_PCPS/toplevel_theorems.v
@@ -4,11 +4,11 @@ Require Import Coq.NArith.BinNat Coq.Relations.Relations Coq.MSets.MSets Coq.MSe
 
 Require Import L6.cps L6.eval L6.cps_util L6.identifiers L6.ctx L6.set_util
         L6.Ensembles_util L6.List_util L6.size_cps L6.tactics L6.relations L6.rel_comp
-        L6.uncurry L6.bounds L6.shrink_cps L6.shrink_cps_toplevel
+        L6.uncurry L6.uncurry_proto L6.bounds L6.shrink_cps L6.shrink_cps_toplevel
         L6.closure_conversion L6.closure_conversion_util L6.hoisting
-        L6.lambda_lifting L6.lambda_lifting_correct.
+        L6.lambda_lifting L6.lambda_lifting_correct L6.uncurry_correct.
 Require Export L6.logical_relations L6.logical_relations_cc L6.alpha_conv
-        L6.inline_letapp L6.inline L6.inline_correct L6.algebra.
+        L6.inline_letapp L6.inline L6.inline_correct L6.algebra L6.state.
 Require Import Common.compM.
 Require Import compcert.lib.Coqlib.
 
@@ -17,34 +17,63 @@ Import ListNotations.
 Close Scope Z_scope.
 
 
-(* TODO use John's definition once merged *)
 
 (* TODO Make tranformations take all parameters first and exp and comp_data last.
         then write correctness theorem as defintion. 
  *) 
 
-Definition well_scoped e :=
-  unique_bindings e /\ Disjoint _ (bound_var e) (occurs_free e).
+Section ToplevelTheorems.
 
-Definition wf_pres e1 e2 :=
-  occurs_free e2 \subset occurs_free e1.
+  Context (cenv : ctor_env).
+  Context (clo_tag : ctor_tag).
+  
+  (* TODO use John's definition  *)
+  Definition well_scoped e :=
+    unique_bindings e /\ Disjoint _ (bound_var e) (occurs_free e).
+  
+  Definition fv_pres e1 e2 :=
+    occurs_free e2 \subset occurs_free e1.
 
-Definition PostT := @PostT nat (nat * nat).
-Definition PostGT := @PostGT nat (nat * nat).
+
+  Definition post_prop P1 PG :=
+    Post_properties cenv P1 P1 PG /\
+    post_upper_bound P1.  
+
+  (** Correctness spec for (composition of) "identity transformations" *)
+
+  Definition correct (trans :  exp -> comp_data -> error exp * comp_data) := 
+    forall e c,
+      well_scoped e ->                                            (* src is well-scoped *)
+      max_var e 1 < state.next_var c ->                           (* the pool of identifiers is fresh *)
+      exists (e' : exp) (c' : state.comp_data),     
+        trans e c = (Ret e', c') /\                               (* the transformation successfully terminates *)
+        well_scoped e' /\                                         (* trg is well-scoped *)
+        max_var e' 1 < state.next_var c' /\                       (* the pool of identifiers is fresh for the target *)
+        exists n, preord_exp_n cenv wf_pres post_prop n e e'.     (* src and trg are in the logical relation  *)
+
+  (** Correctness spec for closure conversion tranformations *)
+
+  Definition correct_cc (trans : exp -> comp_data ->  error exp * comp_data) :=
+    forall e c,
+      well_scoped e ->                                            (* src is well-scoped *)
+      max_var e 1 < state.next_var c ->                           (* the pool of identifiers is fresh *)
+      exists (e' : exp) (c' : state.comp_data),     
+        trans e c = (Ret e', c') /\                               (* the transformation successfully terminates *)
+        well_scoped e' /\                                         (* trg is well-scoped *)
+        max_var e' 1 < state.next_var c' /\                       (* the pool of identifiers is fresh for the target *)
+        exists n m,  R_n_exp cenv clo_tag wf_pres post_prop       (* src and trg are in the logical relation  *)
+                             (simple_bound 0) (simple_bound 0) n m e e'.
+  
 
   
-Context (cenv : ctor_env) (ctag : ctor_tag).
 
-Definition post_prop P1 PG :=
-  Post_properties cenv P1 P1 PG /\
-  post_upper_bound P1.  
 
 Section Inline.
 
  Lemma inline_correct St IH e d st c z :
    well_scoped e ->
    exists (e' : exp) (c' : state.comp_data) click,
-     inline_top' St IH z e d st c true = (Ret e', c', click) /\
+     inline_top' St IH z d st e c = (Ret e', c', click) /\
      wf_pres e e' /\
      well_scoped e' /\
      max_var e' 1 < state.next_var c' /\
@@ -70,22 +99,17 @@ Section Inline.
  Qed.
 
 
- Corollary inline_correct_cor St IH e d st c z :
-   well_scoped e ->
-   max_var e 1 < state.next_var c ->
-   exists (e' : exp) (c' : state.comp_data),
-     inline_top St IH z e d st c true = (Ret e', c') /\
-     well_scoped e' /\
-     max_var e' 1 < state.next_var c' /\
-     preord_exp_n cenv wf_pres post_prop 1 e e'.
+ Corollary inline_correct_cor St IH d st z :
+   correct (inline_top St IH z d st).
  Proof.
-   intros.
+   intro; intros.
    edestruct inline_correct; eauto. destructAll.
    do 2 eexists. split.
    
    unfold inline_top. rewrite H1. reflexivity.
    repeat (split; [ eassumption | ]).
-   econstructor. now eauto. eassumption. split.
+   eexists. econstructor. now eauto. eassumption.
+   split.
    unfold inline_bound_top. eapply inline_bound_compat. omega.
    eapply inline_bound_post_upper_bound.
  Qed.
@@ -101,7 +125,7 @@ Section LambdaLift.
    well_scoped e ->
    max_var e 1 < state.next_var c ->
    exists (e' : exp) (c' : state.comp_data),
-     lambda_lift e k l b c = (Ret e', c') /\
+     lambda_lift k l b e c = (Ret e', c') /\
      max_var e' 1 < state.next_var c' /\
      wf_pres e e' /\
      well_scoped e'  /\
@@ -133,21 +157,15 @@ Section LambdaLift.
       eassumption.
   Qed.
 
-  Corollary lambda_lift_correct_corr e c k l b :
-   well_scoped e ->
-   max_var e 1 < state.next_var c ->
-   exists (e' : exp) (c' : state.comp_data),
-     lambda_lift e k l b c = (Ret e', c') /\
-     max_var e' 1 < state.next_var c' /\
-     well_scoped e'  /\
-     preord_exp_n cenv wf_pres post_prop 1 e e'.
+  Corollary lambda_lift_correct_corr k l b :
+    correct (lambda_lift k l b).
   Proof.
-    intros.
-   edestruct lambda_lift_correct; eauto. destructAll.
-   do 2 eexists. repeat (split; [ eassumption | ]).
-   econstructor. now eauto. eassumption. split.
-   eapply ll_bound_compat. eapply simple_bound_post_upper_bound.
- Qed.
+    intro; intros.
+    edestruct lambda_lift_correct; eauto. destructAll.
+    do 2 eexists. repeat (split; [ eassumption | ]).
+    eexists. econstructor. now eauto. eassumption. split.
+    eapply ll_bound_compat. eapply simple_bound_post_upper_bound.
+  Qed.
 
 
   
@@ -172,7 +190,7 @@ Section Refl.
   
   Context (wf_pres : exp -> exp -> Prop)
           (wf_pres_refl : forall e, wf_pres e e)
-          (cenv : ctor_env) (lf : var).
+          (lf : var).
   
   Context (fuel trace : Type)  {Hf : @fuel_resource fuel} {Ht : @trace_resource trace}.
 
@@ -190,18 +208,11 @@ End Refl.
   
 Section CCHoist.
 
-  Context (clo_tag : ctor_tag).
 
-  Lemma closure_conversion_hoist_correct e c :
-   well_scoped e ->
-   max_var e 1 < state.next_var c ->
-   exists (e' : exp) (c' : state.comp_data),
-     closure_conversion_hoist clo_tag e c = (compM.Ret e', c') /\
-     well_scoped e' /\
-     max_var e' 1 < state.next_var c' /\
-     R_n_exp cenv clo_tag wf_pres post_prop (simple_bound 0) (simple_bound 0) 1%nat 1%nat e e'.
-  Proof.
-    intros Hws Hmvar.
+  Lemma closure_conversion_hoist_correct :
+    correct_cc (closure_conversion_hoist clo_tag).
+  Proof. 
+    intros e c Hws Hmvar.
     edestruct closure_conversion_correct.exp_closure_conv_correct
       with (boundL := simple_bound) (boundG := simple_bound 0).
     (* CC bounds *)
@@ -233,7 +244,7 @@ Section CCHoist.
       + intros. eapply hoisting_bound_mon. eassumption.
       + intros. eapply hoisting_bound_post_Efun_l.
       + intros. eapply hoisting_bound_post_Efun_r. eassumption.
-      + eapply hoisting_bound_compat; eauto. exact (M.empty _).
+      + eapply hoisting_bound_compat; eauto.
       + intros. eapply hoisting_bound_mon. eassumption.
       + reflexivity.
       (* scoping *)
@@ -246,7 +257,7 @@ Section CCHoist.
         * split. eassumption. sets.
         * eapply Pos.le_lt_trans; [| eassumption ].
           eapply max_var_le. eapply Included_Union_compat. eassumption. eassumption.
-        * eexists. split.
+        * do 2 eexists. econstructor. split.
           ++ eapply preord_exp_n_refl.
              clear; firstorder.
           ++ eexists. split. split.
@@ -304,22 +315,16 @@ Section Shrink.
   Qed.
 
 
-  Corollary shrink_err_correct e c :
-   well_scoped e ->
-   max_var e 1 < state.next_var c ->
-   exists (e' : exp) (c' : state.comp_data) (n m : nat),
-     shrink_err e c = (exceptionMonad.Ret (e', n), c') /\ (* TODO change Ret, remove existentials *)
-     max_var e' 1 < state.next_var c' /\
-     well_scoped e' /\
-     preord_exp_n cenv wf_pres post_prop m e e'.
+  Corollary shrink_err_correct :
+    correct shrink_err.
   Proof.
-    intros.
+    intro; intros.
     destruct (shrink_top e) eqn:Hres. 
-    exists e0, c, n.
+    exists e0, c.
     edestruct shrink_top_correct; eauto. destructAll.
-    eexists. split.
+    eexists.
+    unfold shrink_err.
     unfold shrink_err. rewrite Hres. reflexivity.
-    
     split; [| split ]; eauto.
 
     eapply Pos.le_lt_trans. eapply max_var_le. 2: eassumption.
@@ -333,16 +338,10 @@ End Shrink.
 Section InlineLoop.
 
 
-  Lemma inline_loop_correct St IH e d st c z :
-    well_scoped e ->
-    max_var e 1 < state.next_var c ->
-    exists (e' : exp) (c' : state.comp_data),
-      inline_loop St IH z e d st c true = (Ret e', c') /\
-      well_scoped e' /\
-      max_var e' 1 < state.next_var c' /\
-      exists m, preord_exp_n cenv wf_pres post_prop m e e'.
+  Lemma inline_loop_correct z bound d :
+    correct (inline_shrink_loop z bound d).
   Proof.
-    unfold inline_loop.
+    intros e c. unfold inline_shrink_loop, inline_loop.
     revert e c. generalize 1000%nat.
     induction n; intros.
    - simpl. do 2 eexists.
@@ -383,12 +382,54 @@ Section InlineLoop.
 
 End InlineLoop.
 
-(* Section Uncurry. *)
-
-(*   boun *)
+Section Uncurry.
   
-(*   Lemma uncurry_fuel_correct cps n e c :  *)
-(*     uncurry_fuel cps n e st =  -> *)
-(*     forall rho rho1, *)
-(*       preord_env_P cenv PostG (occurs_free e) k rho rho1 -> *)
-(*       preord_exp cenv Post PostG k (e, rho) (e1, rho1). *)
+  Lemma uncurry_top_correct e c b :
+   well_scoped e ->
+   max_var e 1 < state.next_var c ->
+   exists (e' : exp) (c' : state.comp_data),
+     uncurry_top b e c = (Ret e', c') /\
+     max_var e' 1 < state.next_var c' /\
+     wf_pres e e' /\
+     well_scoped e'  /\
+     (forall (k : nat) (rho1 rho2 : env),
+         preord_env_P cenv (simple_bound 0) (occurs_free e) k rho1 rho2 ->
+         binding_in_map (occurs_free e) rho1 ->
+         preord_exp cenv (simple_bound 0) (simple_bound 0) k (e, rho1) (e', rho2)).
+  Proof.
+    intros.
+    edestruct (@uncurry_correct_top cenv nat _ (nat * nat) _ (simple_bound 0)
+                                    (simple_bound 0)) with (cps := b).   
+    - intros. eapply simple_bound_compat.
+    - intros. eapply simple_bound_compat.
+    - eapply Hpost_curry.
+    - eapply Hpost_idemp.
+    - clear. firstorder.
+    - inv H. eassumption.
+    - inv H. eassumption.
+    - eassumption.
+    - destructAll. exists x, x0.
+      split. admit. (* ?? *)
+      split. eassumption.
+      split. eassumption.
+      split. split; eassumption. 
+      now eauto.
+  Admitted.
+
+  Corollary uncurry_top_correct_corr b :
+    correct (uncurry_top b).
+  Proof.
+    intro; intros.
+    edestruct uncurry_top_correct. eassumption. eassumption.
+    destructAll.
+    do 2 eexists. split.
+    admit. (* ?? *)
+    repeat (split; [ eassumption | ]).
+    eexists. econstructor. now eauto. eassumption. split.
+    eapply simple_bound_compat. eapply simple_bound_post_upper_bound.
+
+    Unshelve. eassumption.
+  Admitted.
+
+
+End Uncurry.
