theories/L6_PCPS/toplevel.v
@@ -65,7 +65,7 @@ Definition compile_L6_ANF : CertiCoqTrans toplevel.L4Term L6_FullTerm :=
         (fun (p : toplevel.L4Term) =>
            match convert_top_anf fun_fun_tag default_ctor_tag default_ind_tag p with
            | (compM.Ret e, data) =>
-              let (_, ctag, itag, ftag, cenv, fenv, nenv, _) := data in
+              let (_, ctag, itag, ftag, cenv, fenv, nenv, _, _) := data in
               Ret (M.empty _, cenv, ctag, itag, nenv, fenv, M.empty _, e)
            | (compM.Err s, _) => Err s
            end) src.
@@ -107,14 +107,10 @@ with add_binders_fundefs (names : cps_util.name_env) (B : fundefs) : cps_util.na
 
   Definition log_prog (e : exp) (c_data : comp_data) : comp_data :=
   match c_data with
-  | mkCompData nv nc ni nf cenv fenv nenv log =>
+  | mkCompData nv nc ni nf cenv fenv nenv imap log =>
     let msg := cps_show.show_exp nenv cenv false e in
-    mkCompData nv nc ni nf cenv fenv nenv ("term" :: msg :: log)      
+    mkCompData nv nc ni nf cenv fenv nenv imap ("term" :: msg :: log)      
   end.
-
-  (* Note : To keep the name map small the inliner (which does alpha conversion) will delete mappings of old variables.
-   * To print the ANF term before inlining, the corresponding name environment must be used
-   *)
 
 
   
@@ -149,27 +145,27 @@ with add_binders_fundefs (names : cps_util.name_env) (B : fundefs) : cps_util.na
           let next_var :=
               ((identifiers.max_var e0 1) + 1)%positive in
           let next_fun_tag := M.fold (fun cm => fun ft => fun _ => Pos.max cm ft) fenv 1 + 1 in
-          pack_data next_var ctag itag next_fun_tag cenv fenv nenv nil
+          pack_data next_var ctag itag next_fun_tag cenv fenv nenv (M.empty nat) nil
       in
       let res : error (exp * comp_data):=
           (* Apply ANF transformations *)
           (* Shrink reduction *)
           let (e, _) := time_anf "Shrink" (fun _ => shrink_cps.shrink_top e0) in
           (* Uncurring *)
-          let '(e_err, (_, s), c_data) := time_anf "Uncurry" (fun _ => uncurry_top cps c_data e) in
+          let '(e_err, c_data) := time_anf "Uncurry" (fun _ => uncurry_top cps e c_data) in
           (* let '(e_err, s, c_data) := time_anf "Uncurry" (fun _ => uncurry_fuel cps 100 e c_data) in *)
           e <- e_err ;;
           (* Inlining *)
-          let (e_err, c_data) := time_anf "Inline uncurry wrappers" (fun _ => inline_uncurry next_var e s 10 100 c_data) in
+          let (e_err, c_data) := time_anf "Inline uncurry wrappers" (fun _ => inline_uncurry next_var 10 100 e c_data) in
           e <- e_err ;;
           (* Inline small functions *) 
-          let (e_err, c_data) := if inl_before then time_anf "Inline/shrink loop" (fun _ => inline_small next_var e s 10 100 c_data) else (compM.Ret e, c_data) in
+          let (e_err, c_data) := if inl_before then time_anf "Inline/shrink loop" (fun _ => inline_shrink_loop next_var 10 100 e c_data) else (compM.Ret e, c_data) in
           e <- e_err ;;
           (* Shrink reduction *)
           let (e, _) := time_anf "Shrink" (fun _ => shrink_cps.shrink_top e) in
           (* lambda lifting *)
           let (e_rr, c_data) := if ((opt =? 1)%nat)%bool then
-                                  time_anf "Lambda lift" (fun _ => lambda_lift e args no_push inl_wrappers c_data) 
+                                  time_anf "Lambda lift" (fun _ => lambda_lift args no_push inl_wrappers e c_data) 
                                 else (compM.Ret e, c_data) in
           e <- e_rr ;;
           (* Shrink reduction *)
@@ -177,11 +173,11 @@ with add_binders_fundefs (names : cps_util.name_env) (B : fundefs) : cps_util.na
           (* Closure conversion *)
           let (e_err, c_data) := time_anf "Closure conversion and hoisting"
                                           (fun _ => hoisting.closure_conversion_hoist bogus_closure_tag (* bogus_cloind_tag *) e c_data) in
-          let '(mkCompData next ctag itag ftag cenv fenv names log) := c_data in
           e <- e_err ;;
+          let '(mkCompData next ctag itag ftag cenv fenv names imap log) := c_data in
           let c_data :=
               let cc_var := ((identifiers.max_var e 1) + 1)%positive in (* ΧΧΧ check why this is needed *)
-              pack_data cc_var ctag itag ftag (add_closure_tag bogus_closure_tag bogus_cloind_tag cenv) fenv (add_binders_exp names e) log
+              pack_data cc_var ctag itag ftag (add_closure_tag bogus_closure_tag bogus_cloind_tag cenv) fenv (add_binders_exp names e) imap log
           in
           (* Shrink reduction *)
           let (e, _) := time_anf "Shrink" (fun _ => shrink_cps.shrink_top e) in
@@ -193,12 +189,12 @@ with add_binders_fundefs (names : cps_util.name_env) (B : fundefs) : cps_util.na
           (* Shrink reduction *)
           let (e, _) := time_anf "Shrink" (fun _ => shrink_cps.shrink_top e) in
           (* Inline small functions *) 
-          let (e_err, c_data) := if inl_after then time_anf "Inline/shrink loop" (fun _ => inline_small next_var e s 10 100 c_data) else (compM.Ret e, c_data) in
+          let (e_err, c_data) := if inl_after then time_anf "Inline/shrink loop" (fun _ => inline_shrink_loop next_var 10 100 e c_data) else (compM.Ret e, c_data) in
           e <- e_err ;;
           (* Inline in wrapper functions *)
           let (e_err, c_data) := if inl_known then
                                    let (e, _) := time_anf "Shrink" (fun _ => shrink_cps.shrink_top e) in
-                                   time_anf "Inline known functions inside wrappers" (fun _ => inline_lifted next_var e s 10 1000 c_data)
+                                   time_anf "Inline known functions inside wrappers" (fun _ => inline_lifted next_var e 10 1000 c_data)
                                  else (compM.Ret e, c_data) in
           e <- e_err ;;
 
@@ -208,10 +204,10 @@ with add_binders_fundefs (names : cps_util.name_env) (B : fundefs) : cps_util.na
       | compM.Err s =>
         (Err ("Failed compiling L6 program: " ++ s)%string, "")
       | compM.Ret (e, c_data) =>
-        let (_, ctag, itag, ftag, cenv, fenv, nenv, log) := c_data in
+        let (_, ctag, itag, ftag, cenv, fenv, nenv, _, log) := c_data in
         (Ret (prims, cenv, ctag, itag, nenv, fenv, M.empty _, e), log_to_string log)
       end.
-
+    
 
     (* Just for debugging *)
     Definition L6_pipeline_print (t : L6_FullTerm) : error L6_FullTerm * string :=
@@ -221,27 +217,27 @@ with add_binders_fundefs (names : cps_util.name_env) (B : fundefs) : cps_util.na
           let next_var :=
               ((identifiers.max_var e0 1) + 1)%positive in
           let next_fun_tag := M.fold (fun cm => fun ft => fun _ => Pos.max cm ft) fenv 1 + 1 in
-          pack_data next_var ctag itag next_fun_tag cenv fenv nenv nil
+          pack_data next_var ctag itag next_fun_tag cenv fenv nenv (M.empty _) nil
       in
       let res : error (exp * comp_data):=
           (* Apply ANF transformations *)
           (* Shrink reduction *)
           let (e, _) := time_anf "Shrink" (fun _ => shrink_cps.shrink_top e0) in
           (* Uncurring *)
-          let '(e_err, (_, s), c_data) := time_anf "Uncurry" (fun _ => uncurry_top cps c_data e) in
+          let '(e_err, c_data) := time_anf "Uncurry" (fun _ => uncurry_top cps e c_data) in
           (* let '(e_err, s, c_data) := time_anf "Uncurry" (fun _ => uncurry_fuel cps 100 e c_data) in *)
           e <- e_err ;;
           (* Inlining *)
-          let (e_err, c_data) := time_anf "Inline uncurry wrappers" (fun _ => inline_uncurry next_var e s 10 100 c_data) in
+          let (e_err, c_data) := time_anf "Inline uncurry wrappers" (fun _ => inline_uncurry next_var 10 100 e c_data) in
           e <- e_err ;;
           (* Inline small functions *) 
-          let (e_err, c_data) := time_anf "Inline/shrink loop" (fun _ => inline_small next_var e s 10 100 c_data) in
+          let (e_err, c_data) := time_anf "Inline/shrink loop" (fun _ => inline_shrink_loop next_var 10 100 e c_data) in
           e <- e_err ;;
           (* Shrink reduction *)
           let (e, _) := time_anf "Shrink" (fun _ => shrink_cps.shrink_top e) in
           (* lambda lifting *)
           let (e_rr, c_data) := if ((opt =? 1)%nat)%bool then
-                                  time_anf "Lambda lift" (fun _ => lambda_lift e args no_push inl_wrappers c_data) 
+                                  time_anf "Lambda lift" (fun _ => lambda_lift args no_push inl_wrappers e c_data) 
                                 else (compM.Ret e, c_data) in
 
           ret (e, c_data)
@@ -250,7 +246,7 @@ with add_binders_fundefs (names : cps_util.name_env) (B : fundefs) : cps_util.na
       | compM.Err s =>
         (Err ("Failed compiling L6 program: " ++ s)%string, "")
       | compM.Ret (e, c_data) =>
-        let (_, ctag, itag, ftag, cenv, fenv, nenv, log) := c_data in
+        let (_, ctag, itag, ftag, cenv, fenv, nenv, _, log) := c_data in
         (Ret (prims, cenv, ctag, itag, nenv, fenv, M.empty _, e), log_to_string log)
       end.
 
